protocols/PORExtended.v
@@ -81,6 +81,29 @@ Proof.
   invert H6.
 Qed.
 
+Lemma syntactically_safe_U_preservation_step :
+  forall t__hon t__adv (st st' : universe t__hon t__adv * IdealWorld.universe t__hon) b,
+    step st st'
+    -> lameAdv b (fst st).(adversary)
+    -> goodness_predicates (fst st)
+    -> syntactically_safe_U (fst st)
+    -> syntactically_safe_U (fst st').
+Proof.
+  inversion 1; intros; subst; simpl in *; eapply syntactically_safe_U_preservation_stepU; eauto.
+Qed.
+
+Lemma syntactically_safe_U_preservation_steps :
+  forall t__hon t__adv st st' b,
+    (@step t__hon t__adv) ^* st st'
+    -> lameAdv b (fst st).(adversary)
+    -> goodness_predicates (fst st)
+    -> syntactically_safe_U (fst st)
+    -> syntactically_safe_U (fst st').
+Proof.
+  induction 1; intros; eauto.
+  eapply IHtrc; eauto using syntactically_safe_U_preservation_step, goodness_preservation_step.
+Qed.
+
 Lemma stuck_model_step_user_stuck_user_implies_labels_align :
   forall t__hon t__adv st,
     @stuck_model_step_user_stuck_user t__hon t__adv st
@@ -529,18 +552,19 @@ Module ProtocolSimulates (Proto : SyntacticallySafeProtocol).
   Qed.
 
   Lemma ss_implies_next_safe :
-    forall t (cmd : user_cmd t) uid ctx sty honestk cs froms sents,
-      syntactically_safe uid ctx cmd sty
-      -> typingcontext_sound ctx honestk cs uid
+    forall t (cmd : user_cmd t) uid ctx uids sty cs,
+      syntactically_safe uid uids ctx cmd sty
       -> forall A B (usrs usrs' : honest_users A) (adv adv' : user_data B) cmd'
-          cs' gks gks' ks ks' qmsgs qmsgs' mycs mycs' froms' sents' n n' lbl,
-          step_user lbl (Some uid)
-                    (usrs,adv,cs,gks,ks,qmsgs,mycs,froms,sents,n,cmd)
-                    (usrs',adv',cs',gks',ks',qmsgs',mycs',froms',sents',n',cmd')
-          -> forall t__n (cmd__n : user_cmd t__n), nextAction cmd cmd__n
-          -> (forall r, cmd__n <> Return r)
-          -> no_resends sents'
-          -> next_cmd_safe honestk cs uid froms sents cmd.
+          cs' gks gks' ks ks' qmsgs qmsgs' mycs mycs' froms froms' sents sents' n n' lbl,
+        step_user lbl (Some uid)
+                  (usrs,adv,cs,gks,ks,qmsgs,mycs,froms,sents,n,cmd)
+                  (usrs',adv',cs',gks',ks',qmsgs',mycs',froms',sents',n',cmd')
+        -> typingcontext_sound ctx usrs cs uid
+        -> uids = compute_ids usrs
+        -> forall t__n (cmd__n : user_cmd t__n), nextAction cmd cmd__n
+        -> (forall r, cmd__n <> Return r)
+        -> no_resends sents'
+        -> next_cmd_safe (findUserKeys usrs) cs uid froms sents cmd.
   Proof.
     induct cmd;
       unfold next_cmd_safe; intros;
@@ -549,20 +573,20 @@ Module ProtocolSimulates (Proto : SyntacticallySafeProtocol).
         end; eauto;
           try solve [ unfold typingcontext_sound in *; split_ex;
                       match goal with
-                      | [ H : syntactically_safe _ _ _ _ |- _ ] => invert H
+                      | [ H : syntactically_safe _ _ _ _ _ |- _ ] => invert H
                       end; eauto ].
 
     - invert H0.
-      invert H2; eauto.
-      invert H3.
+      invert H1; eauto.
+      invert H4.
       eapply IHcmd in H8; eauto.
-      eapply H8 in H10; eauto.
+      eapply H8 in H11; eauto.
 
-      invert H3. invert H7. specialize (H4 a0); contradiction.
+      invert H11; trivial.
 
     - unfold typingcontext_sound in *; split_ex; invert H.
-      apply H5 in H12; split_ex; subst.
-      apply H0 in H10.
+      apply H2 in H11; split_ex; subst.
+      apply H1 in H10.
       unfold msg_honestly_signed, msg_signing_key,
              msg_to_this_user, msg_destination_user,
              msgCiphersSignedOk, honest_keyb;
@@ -574,23 +598,24 @@ Module ProtocolSimulates (Proto : SyntacticallySafeProtocol).
         context_map_rewrites;
         trivial.
       (do 2 eexists); repeat simple apply conj; eauto.
-      invert H1.
-      unfold no_resends, updateSentNonce in H4; context_map_rewrites.
+      invert H0.
+      unfold no_resends, updateSentNonce in H5; context_map_rewrites.
       destruct (cipher_to_user x0 ==n cipher_to_user x0); try contradiction.
-      invert H4; eauto.
+      invert H5; eauto.
       
     - unfold typingcontext_sound in *; split_ex; invert H; eauto.
       intros.
-      apply H14 in H; split_ex; subst; eauto.
+      apply H12 in H; split_ex; subst; eauto.
   Qed.
 
   Lemma ss_implies_next_safe_not_send :
-    forall t (cmd : user_cmd t) uid ctx sty honestk cs froms sents,
-      syntactically_safe uid ctx cmd sty
-      -> typingcontext_sound ctx honestk cs uid
+    forall t (cmd : user_cmd t) {A} (usrs : honest_users A) uid uids ctx sty cs froms sents,
+      syntactically_safe uid uids ctx cmd sty
+      -> typingcontext_sound ctx usrs cs uid
+      -> uids = compute_ids usrs
       -> forall t__n (cmd__n : user_cmd t__n), nextAction cmd cmd__n
       -> (forall t__msg recuid (msg : crypto t__msg), cmd__n ~= Send recuid msg -> False)
-      -> next_cmd_safe honestk cs uid froms sents cmd.
+      -> next_cmd_safe (findUserKeys usrs) cs uid froms sents cmd.
   Proof.
     induct cmd;
       unfold next_cmd_safe; intros;
@@ -599,38 +624,36 @@ Module ProtocolSimulates (Proto : SyntacticallySafeProtocol).
         end; eauto;
           try solve [ unfold typingcontext_sound in *; split_ex;
                       match goal with
-                      | [ H : syntactically_safe _ _ _ _ |- _ ] => invert H
+                      | [ H : syntactically_safe _ _ _ _ _ |- _ ] => invert H
                       end; eauto ].
 
     - invert H0.
-      invert H2; eauto.
-      eapply IHcmd in H11; eauto.
-      eapply na_deterministic in H8; eauto; split_ex; subst.
+      invert H3; eauto.
+      eapply IHcmd with (froms := froms) (sents := sents) in H11; eauto.
+      eapply na_deterministic in H9; eauto; split_ex; subst.
       invert H2.
       eapply H11 in H6; eauto.
 
-    - invert H1.
+    - invert H2.
       exfalso.
-      eapply H2; eauto.
+      eapply H3; eauto.
       
     - unfold typingcontext_sound in *; split_ex; invert H; eauto.
       intros.
-      apply H12 in H; split_ex; subst; eauto.
-
-      Unshelve.
-      eauto.
+      apply H10 in H; split_ex; subst; eauto.
   Qed.
 
   Lemma ss_implies_next_safe_not_send' :
-    forall t (cmd : user_cmd t) uid ctx sty honestk cs froms sents,
-      syntactically_safe uid ctx cmd sty
-      -> typingcontext_sound ctx honestk cs uid
+    forall t (cmd : user_cmd t) uid uids ctx sty A (usrs : honest_users A) cs froms sents,
+      syntactically_safe uid uids ctx cmd sty
+      -> typingcontext_sound ctx usrs cs uid
+      -> uids = compute_ids usrs
       -> forall t__n (cmd__n : user_cmd t__n), nextAction cmd cmd__n
       -> match cmd__n with
         | Send recuid msg => t__n = Base Unit /\ (cmd__n ~= Send recuid msg -> False)
         | _ => False
         end
-      -> next_cmd_safe honestk cs uid froms sents cmd.
+      -> next_cmd_safe (findUserKeys usrs) cs uid froms sents cmd.
   Proof.
     induct cmd;
       unfold next_cmd_safe; intros;
@@ -639,65 +662,24 @@ Module ProtocolSimulates (Proto : SyntacticallySafeProtocol).
         end; eauto;
           try solve [ unfold typingcontext_sound in *; split_ex;
                       match goal with
-                      | [ H : syntactically_safe _ _ _ _ |- _ ] => invert H
+                      | [ H : syntactically_safe _ _ _ _ _ |- _ ] => invert H
                       end; eauto ].
 
     - invert H0.
-      invert H2; eauto.
-      eapply IHcmd in H11; eauto.
-      eapply na_deterministic in H8; eauto; split_ex; subst.
+      invert H3; eauto.
+      eapply IHcmd with (froms := froms) (sents := sents) in H11; eauto.
+      eapply na_deterministic in H9; eauto; split_ex; subst.
       invert H2.
       eapply H11 in H6; eauto.
 
-    - invert H1.
+    - invert H2; split_ex.
       exfalso.
       eapply H2; eauto.
       
     - unfold typingcontext_sound in *; split_ex; invert H; eauto.
       intros.
-      apply H12 in H; split_ex; subst; eauto.
-
-      Unshelve.
-      eauto.
+      apply H10 in H; split_ex; subst; eauto.
   Qed.
-
-  (* Lemma ss_implies_next_safe_not_send : *)
-  (*   forall t__hon t__adv (usrs : honest_users t__hon)  (cmd : user_cmd t) uid ctx sty honestk cs froms sents, *)
-  (*     syntactically_safe uid ctx cmd sty *)
-  (*     -> typingcontext_sound ctx honestk cs uid *)
-  (*     -> forall t__n (cmd__n : user_cmd t__n), nextAction cmd cmd__n *)
-  (*     -> next_cmd_safe honestk cs uid froms sents cmd. *)
-  (* Proof. *)
-  (*   induct cmd; *)
-  (*     unfold next_cmd_safe; intros; *)
-  (*       match goal with *)
-  (*       | [ H : nextAction _ _ |- _ ] => invert H *)
-  (*       end; eauto; *)
-  (*         try solve [ unfold typingcontext_sound in *; split_ex; *)
-  (*                     match goal with *)
-  (*                     | [ H : syntactically_safe _ _ _ _ |- _ ] => invert H *)
-  (*                     end; eauto ]. *)
-
-  (*   - invert H0. *)
-  (*     invert H2; eauto. *)
-  (*     eapply IHcmd in H11; eauto. *)
-  (*     eapply na_deterministic in H8; eauto; split_ex; subst. *)
-  (*     invert H2. *)
-  (*     eapply H11 in H6; eauto. *)
-
-  (*   - invert H1. *)
-  (*     exfalso. *)
-  (*     eapply H2; eauto. *)
-      
-  (*   - unfold typingcontext_sound in *; split_ex; invert H; eauto. *)
-  (*     intros. *)
-  (*     apply H12 in H; split_ex; subst; eauto. *)
-
-  (*     Unshelve. *)
-  (*     eauto. *)
-  (* Qed. *)
-
-  
 
   Lemma model_step_implies_step :
     forall t__hon t__adv uid st st',
@@ -731,151 +713,109 @@ Module ProtocolSimulates (Proto : SyntacticallySafeProtocol).
     intros; subst; eapply StepBindRecur; eauto.
   Qed.
 
-  (* Lemma step_na_not_return : *)
+  Lemma syntactically_safe_na :
+    forall t (cmd : user_cmd t) t__n (cmd__n : user_cmd t__n),
+      nextAction cmd cmd__n
+      -> forall ctx uid uids styp,
+        syntactically_safe uid uids ctx cmd styp
+        -> exists styp',
+          syntactically_safe uid uids ctx cmd__n styp'.
+  Proof.
+    induction 1; eauto.
+    intros * SS; invert SS; eauto.
+  Qed.
+
+
+  (* Lemma step_na_recur : *)
   (*   forall t t__n (cmd : user_cmd t) (cmd__n : user_cmd t__n), *)
   (*     nextAction cmd cmd__n *)
-                 
-  (*     -> forall A B uid lbl bd bd' cs cs' (usrs usrs': honest_users A) (adv adv' : user_data B) gks gks' *)
-  (*         cmd__n' ks ks' qmsgs qmsgs' mycs mycs' *)
-  (*         froms froms' sents sents' cur_n cur_n' , *)
+  (*     -> (forall r, cmd__n <> Return r) *)
+  (*     -> forall A B suid lbl bd bd', *)
 
-  (*       step_user lbl (Some uid) bd bd' *)
-  (*       -> bd = (usrs, adv, cs, gks, ks, qmsgs, mycs, froms, sents, cur_n, cmd__n) *)
-  (*       -> bd' = (usrs', adv', cs', gks', ks', qmsgs', mycs', froms', sents', cur_n', cmd__n') *)
-  (*       -> exists f cmd', *)
-  (*           cmd = f cmd__n *)
-  (*           /\ cmd' = f cmd__n' *)
-  (*           /\ forall lbl1 suid1 (usrs1 usrs1' : honest_users A) (adv1 adv1' : user_data B) *)
-  (*               cs1 cs1' gks1 gks1' *)
-  (*               ks1 ks1' qmsgs1 qmsgs1' mycs1 mycs1' cmd__n'' *)
-  (*               froms1 froms1' sents1 sents1' cur_n1 cur_n1', *)
+  (*       step_user lbl suid bd bd' *)
 
-  (*               step_user lbl1 suid1 *)
-  (*                         (usrs1, adv1, cs1, gks1, ks1, qmsgs1, mycs1, froms1, sents1, cur_n1, cmd__n) *)
-  (*                         (usrs1', adv1', cs1', gks1', ks1', qmsgs1', mycs1', froms1', sents1', cur_n1', cmd__n'') *)
-  (*               -> step_user lbl1 suid1 *)
-  (*                           (usrs1, adv1, cs1, gks1, ks1, qmsgs1, mycs1, froms1, sents1, cur_n1, f cmd__n) *)
-  (*                           (usrs1', adv1', cs1', gks1', ks1', qmsgs1', mycs1', froms1', sents1', cur_n1', f cmd__n''). *)
+  (*       -> forall cs cs' (usrs usrs': honest_users A) (adv adv' : user_data B) gks gks' *)
+  (*           cmd__n' ks ks' qmsgs qmsgs' mycs mycs' *)
+  (*           froms froms' sents sents' cur_n cur_n', *)
+
+  (*         bd = (usrs, adv, cs, gks, ks, qmsgs, mycs, froms, sents, cur_n, cmd__n) *)
+  (*         -> bd' = (usrs', adv', cs', gks', ks', qmsgs', mycs', froms', sents', cur_n', cmd__n') *)
+  (*         -> exists bd'', *)
+  (*             step_user lbl suid (usrs, adv, cs, gks, ks, qmsgs, mycs, froms, sents, cur_n, cmd) bd''. *)
   (* Proof. *)
-  (*   induction 1; inversion 2; inversion 1; intros; subst. *)
-  (*   - invert H. *)
-  (*   - exists (fun x => x); eexists; repeat simple apply conj; eauto. *)
-  (*   - exists (fun x => x); eexists; repeat simple apply conj; eauto. *)
-  (*   - exists (fun x => x); eexists; repeat simple apply conj; eauto. *)
-  (*   - exists (fun x => x); eexists; repeat simple apply conj; eauto. *)
-  (*   - exists (fun x => x); eexists; repeat simple apply conj; eauto. *)
-  (*   - exists (fun x => x); eexists; repeat simple apply conj; eauto. *)
-  (*   - exists (fun x => x); eexists; repeat simple apply conj; eauto. *)
-  (*   - exists (fun x => x); eexists; repeat simple apply conj; eauto. *)
-  (*   - exists (fun x => x); eexists; repeat simple apply conj; eauto. *)
-  (*   - clean_context. *)
-  (*     eapply IHnextAction in H0; eauto; split_ex; subst. *)
-  (*     exists (fun CD => x <- x CD; c2 x). *)
-  (*     eexists; subst; repeat simple apply conj; intros; eauto. *)
-  (*     eapply StepBindRecur'. *)
-  (*     remember (Some uid) as suid. *)
-  (*     match goal with *)
-  (*     | [ |- step_user _ _ ?bd1 ?bd2 ] => *)
-  (*       remember bd1 as bbd1; *)
-  (*         remember bd2 as bbd2 *)
-  (*     end. *)
+  (*   induct 1; intros; subst; eauto. *)
+  (*   eapply IHnextAction in H0; eauto. *)
+  (*   split_ex. *)
+  (*   dt x. *)
+  (*   eexists. *)
+  (* Admitted. *)
 
-  
-  (* Lemma step_na_not_return : *)
+
+  Lemma step_na_recur :
+    forall t t__n (cmd : user_cmd t) (cmd__n : user_cmd t__n),
+      nextAction cmd cmd__n
+      -> forall A B suid lbl bd bd',
+
+        step_user lbl suid bd bd'
+
+        -> forall cs cs' (usrs usrs': honest_users A) (adv adv' : user_data B) gks gks'
+            cmd__n' ks ks' qmsgs qmsgs' mycs mycs'
+            froms froms' sents sents' cur_n cur_n',
+
+          bd = (usrs, adv, cs, gks, ks, qmsgs, mycs, froms, sents, cur_n, cmd__n)
+          -> bd' = (usrs', adv', cs', gks', ks', qmsgs', mycs', froms', sents', cur_n', cmd__n')
+          -> exists bd'',
+              step_user lbl suid (usrs, adv, cs, gks, ks, qmsgs, mycs, froms, sents, cur_n, cmd) bd''.
+  Proof.
+    induct 1; intros; subst;
+      eauto.
+
+    eapply IHnextAction in H0; eauto; split_ex; eauto.
+  Admitted.
+
+  (* Lemma step_na_recur : *)
   (*   forall t t__n (cmd : user_cmd t) (cmd__n : user_cmd t__n), *)
   (*     nextAction cmd cmd__n *)
-                 
-  (*     -> forall A B uid lbl bd bd' cs cs' (usrs usrs': honest_users A) (adv adv' : user_data B) gks gks' *)
-  (*         cmd__n' ks ks' qmsgs qmsgs' mycs mycs' *)
-  (*         froms froms' sents sents' cur_n cur_n' , *)
+  (*     -> forall A B suid lbl bd bd', *)
 
-  (*       step_user lbl (Some uid) bd bd' *)
-  (*       -> bd = (usrs, adv, cs, gks, ks, qmsgs, mycs, froms, sents, cur_n, cmd__n) *)
-  (*       -> bd' = (usrs', adv', cs', gks', ks', qmsgs', mycs', froms', sents', cur_n', cmd__n') *)
-  (*       -> exists f cmd', *)
-  (*           cmd = f cmd__n *)
-  (*           /\ cmd' = f cmd__n' *)
-  (*           /\ step_user lbl (Some uid) *)
-  (*                       (usrs, adv, cs, gks, ks, qmsgs, mycs, froms, sents, cur_n, f cmd__n) *)
-  (*                       (usrs', adv', cs', gks', ks', qmsgs', mycs', froms', sents', cur_n', f cmd__n'). *)
+  (*       step_user lbl suid bd bd' *)
+
+  (*       -> forall cs cs' (usrs usrs': honest_users A) (adv adv' : user_data B) gks gks' *)
+  (*           cmd__n' ks ks' qmsgs qmsgs' mycs mycs' *)
+  (*           froms froms' sents sents' cur_n cur_n', *)
+
+  (*         bd = (usrs, adv, cs, gks, ks, qmsgs, mycs, froms, sents, cur_n, cmd__n) *)
+  (*         -> bd' = (usrs', adv', cs', gks', ks', qmsgs', mycs', froms', sents', cur_n', cmd__n') *)
+  (*         -> exists bd'', *)
+  (*             step_user lbl suid (usrs, adv, cs, gks, ks, qmsgs, mycs, froms, sents, cur_n, cmd) bd''. *)
   (* Proof. *)
-  (*   induction 1; inversion 2; inversion 1; intros; subst. *)
-  (*   - invert H. *)
-  (*   - exists (fun x => x); eexists; repeat simple apply conj; eauto. *)
-  (*   - exists (fun x => x); eexists; repeat simple apply conj; eauto. *)
-  (*   - exists (fun x => x); eexists; repeat simple apply conj; eauto. *)
-  (*   - exists (fun x => x); eexists; repeat simple apply conj; eauto. *)
-  (*   - exists (fun x => x); eexists; repeat simple apply conj; eauto. *)
-  (*   - exists (fun x => x); eexists; repeat simple apply conj; eauto. *)
-  (*   - exists (fun x => x); eexists; repeat simple apply conj; eauto. *)
-  (*   - exists (fun x => x); eexists; repeat simple apply conj; eauto. *)
-  (*   - exists (fun x => x); eexists; repeat simple apply conj; eauto. *)
-  (*   - clean_context. *)
-  (*     eapply IHnextAction in H0; eauto; split_ex; subst. *)
-  (*     exists (fun CD => x <- x CD; c2 x). *)
-  (*     eexists; subst; repeat simple apply conj; eauto. *)
-  (*     eapply StepBindRecur'. *)
-  (*     remember (Some uid) as suid. *)
+  (*   induct cmd; intros; subst; *)
   (*     match goal with *)
-  (*     | [ |- step_user _ _ ?bd1 ?bd2 ] => *)
-  (*       remember bd1 as bbd1; *)
-  (*         remember bd2 as bbd2 *)
-  (*     end. *)
+  (*     | [ H : nextAction _ _ |- _ ] => invert H *)
+  (*     end; eauto. *)
 
-      
-  (*     eapply StepBindRecur' with (cmd1 := x c) (cmd1' :=  x cmd__n') (cmd2 := c2). *)
-    
+  (*   invert H0. *)
+
+  (*   eapply IHcmd in H5; eauto; split_ex; eauto. *)
+  (*   exists x. *)
+
+  (* Admitted. *)
 
 
-  (* Lemma step_na_not_return : *)
-  (*   forall {A B C} suid lbl bd bd', *)
-
+  (* Lemma step_na_recur : *)
+  (*   forall {A B C D} suid lbl bd bd', *)
   (*     step_user lbl suid bd bd' *)
 
   (*     -> forall cs cs' (usrs usrs': honest_users A) (adv adv' : user_data B) gks gks' *)
-  (*         (cmd__n cmd__n' : user_cmd C) (cmd : user_cmd (Base A)) ks ks' qmsgs qmsgs' mycs mycs' *)
+  (*         (cmd : user_cmd C) (cmd__n cmd'__n : user_cmd D) ks ks' qmsgs qmsgs' mycs mycs' *)
   (*         froms froms' sents sents' cur_n cur_n', *)
 
   (*       bd = (usrs, adv, cs, gks, ks, qmsgs, mycs, froms, sents, cur_n, cmd__n) *)
-  (*       -> bd' = (usrs', adv', cs', gks', ks', qmsgs', mycs', froms', sents', cur_n', cmd__n') *)
+  (*       -> bd' = (usrs', adv', cs', gks', ks', qmsgs', mycs', froms', sents', cur_n', cmd'__n) *)
   (*       -> nextAction cmd cmd__n *)
-  (*       -> exists f cmd', *)
-  (*           (* step_user lbl suid *) *)
-  (*           (*           (usrs, adv, cs, gks, ks, qmsgs, mycs, froms, sents, cur_n, cmd__n) *) *)
-  (*           (*           (usrs', adv', cs', gks', ks', qmsgs', mycs', froms', sents', cur_n', cmd__n') *) *)
-  (*             cmd = f cmd__n *)
-  (*           /\ cmd' = f cmd__n' *)
-  (*           /\ step_user lbl suid *)
-  (*                       (usrs, adv, cs, gks, ks, qmsgs, mycs, froms, sents, cur_n, f cmd__n) *)
-  (*                       (usrs', adv', cs', gks', ks', qmsgs', mycs', froms', sents', cur_n', f cmd__n'). *)
+  (*       -> exists bd', *)
+  (*           step_user lbl suid (usrs, adv, cs, gks, ks, qmsgs, mycs, froms, sents, cur_n, cmd) bd'. *)
   (* Proof. *)
-  (*   Hint Constructors step_user syntactically_safe : core. *)
-
-  (*   induction 1; inversion 1; inversion 1; intros; subst. *)
-
-  (*   - eapply nextAction_couldBe in H13; contradiction. *)
-  (*   - eapply nextAction_couldBe in H12; contradiction. *)
-  (*   -  *)
-
-
-  (*   - eapply IHstep_user in H28; eauto. *)
-  (*     split_ex. *)
-  (*     exists (fun CD => x <- x CD; cmd2 x). *)
-  (*     eexists; subst; repeat simple apply conj; eauto. *)
-      
-  (*   - invert H27. *)
-  (*     unfold not in *; exfalso; eauto. *)
-  (*   - exists (fun x => x); eexists; repeat simple apply conj; swap 1 3; eauto. *)
-  (*   - exists (fun x => x); eexists; repeat simple apply conj; swap 1 3; eauto. *)
-  (*   - exists (fun x => x); eexists; repeat simple apply conj; swap 1 3; eauto. *)
-  (*   - exists (fun x => x); eexists; repeat simple apply conj; swap 1 3; eauto. *)
-  (*   - exists (fun x => x); eexists; repeat simple apply conj; swap 1 3; eauto. *)
-  (*   - exists (fun x => x); eexists; repeat simple apply conj; swap 1 3; eauto. *)
-  (*   - exists (fun x => x); eexists; repeat simple apply conj; swap 1 3; eauto. *)
-  (*   - exists (fun x => x); eexists; repeat simple apply conj; swap 1 3; eauto. *)
-  (*   - exists (fun x => x); eexists; repeat simple apply conj; swap 1 3; eauto. *)
-  (*   - exists (fun x => x); eexists; repeat simple apply conj; swap 1 3; eauto. *)
-  (* Qed. *)
 
 
   Lemma simsafe : honest_actions_safe t__adv R.
@@ -889,12 +829,21 @@ Module ProtocolSimulates (Proto : SyntacticallySafeProtocol).
     assert ( (ru0,iu0) = (ru0,iu0) \/ False ) as ARG by auto.
     specialize (H0 _ ARG).
 
-    assert (syntactically_safe_U ru) by admit.
+    assert (syntactically_safe_U ru).
+    pose proof universe_starts_safe; simpl in *; split_ex.
+    change (syntactically_safe_U (fst (ru,U__i))).
+    assert (goodness_predicates (fst (ru0, iu0))) by
+        (unfold goodness_predicates , adv_universe_ok, universe_ok in *; intuition idtac).
+
+    eapply syntactically_safe_U_preservation_steps; eauto.
+
+
+    
     unfold syntactically_safe_U in *; simpl in *.
     unfold honest_cmds_safe; intros; subst.
     destruct u; simpl.
     generalize H6; intros USRS; rewrite <- H in USRS.
-    specialize (H4 _ _ USRS); split_ex; simpl in *.
+    specialize (H4 _ _ _ USRS eq_refl); split_ex; simpl in *.
 
     rename U__i into iu.
     red. intros.
@@ -929,117 +878,41 @@ Module ProtocolSimulates (Proto : SyntacticallySafeProtocol).
         specialize (H0 _ eq_refl);
         eauto.
 
-    - dependent destruction cmd__n; eauto.
-      + eapply nextAction_couldBe in H7; contradiction.
+    - eapply syntactically_safe_na in H4; eauto; split_ex.
+      rewrite <- H, <- H1.
+      unfold typingcontext_sound in *; split_ex; invert H4; process_ctx; eauto.
+
+      + eapply nextAction_couldBe in H7; eauto.
+      + apply H13 in H11; split_ex; subst; eauto.
       + exfalso.
         assert (forall st', model_step_user u_id (ru,iu) st' -> False) by eauto using not_ex_all_not.
         pose proof stuck_not_misaligned_inv as NOTMISAL.
         specialize (NOTMISAL _ ARG _ H3).
-        eapply NOTMISAL in H9.
+        eapply NOTMISAL in H11.
         2: simpl; exact USRS.
-
         
         unfold build_data_step in *; simpl in *.
         assert (STEP : exists lbl bd,
                    step_user lbl
                              (Some u_id)
                              (users ru, adversary ru, all_ciphers ru, all_keys ru,
-                              key_heap, msg_heap, c_heap, from_nons, sent_nons, cur_nonce, Send uid msg) bd).
-        (do 2 eexists).
-        econstructor; eauto.
+                              key_heap, msg_heap, c_heap, from_nons, sent_nons, cur_nonce,
+                              Send (cipher_to_user x2) (@SignedCiphertext t0 x1)) bd).
 
-        unfold typingcontext_sound in *.
+        (* generalize (syntactically_safe_na _ _ _ _ H7 _ _ _ _ H4); intros; split_ex. *)
+        unfold typingcontext_sound in *; split_ex.
+        (do 2 eexists); econstructor; clean_map_lookups; simpl in *; eauto.
+        context_map_rewrites; eauto.
+        unfold not; intros INV; invert INV; contradiction.
         
+        split_ex.
 
-        
-        eapply step_na_not_return in H7; eauto.
-        
-        eapply H9.
-        unfold build_data_step; simpl.
+        assert (forall st', model_step_user u_id (ru,iu) st' -> False) by eauto using not_ex_all_not.
+        eapply NOTMISAL in H17; eauto.
+        unfold build_data_step in H17; simpl in H17; eauto.
 
-        
-
-
-    - destruct (classic (forall t__msg recuid (msg : crypto t__msg), cmd__n ~= Send recuid msg -> False)).
-      + eapply ss_implies_next_safe_not_send; eauto.
-        rewrite <- H, <- H1; assumption.
-      + dependent destruction cmd__n; eauto.
-
-      
-
-    - destruct (classic (match cmd__n with
-                         | Send recuid msg => B = Base Unit /\ (cmd__n ~= Send recuid msg -> False)
-                         | _ => False
-                         end)).
-
-      + eapply ss_implies_next_safe_not_send; eauto.
-        rewrite <- H, <- H1; assumption.
-        dependent destruction cmd__n; try contradiction.
-        split_ands; eauto.
-
-      + dependent destruction cmd__n; eauto.
-        * eapply nextAction_couldBe in H7; contradiction.
-        * exfalso.
-          eapply H9.
-          split; intros; eauto.
-          invert
-        
-        
-
-
-      
-    - destruct (classic (forall t__msg recuid (msg : crypto t__msg), cmd__n ~= Send recuid msg -> False)).
-      + eapply ss_implies_next_safe_not_send; eauto.
-        rewrite <- H, <- H1; assumption.
-
-      + exfalso.
-        eapply H9.
-        intros.
-        invert H10.
-
-        
-        
-      
-
-      dependent destruction cmd__n; auto.
-      apply nextAction_couldBe in H7; contradiction.
-      eapply ss_implies_next_safe in H7; eauto.
-
-      
-      (* rewrite Forall_natmap_forall in H0; *)
-      (*   specialize (H0 _ _ USRS). *)
-      (* invert H8; simpl in *. *)
-      (* eapply ss_implies_next_safe; eauto. *)
-      (* unfold next_cmd_safe; intros. *)
-
-      (* induct H8; eauto. *)
-      (* admit. *)
-      (* invert H4. *)
-      (* eapply IHnextAction in H15; eauto. *)
-      
-
-      (* generalize H8; intros NA; apply nextAction_couldBe in NA. *)
-      (* dependent destruction protocol; try contradiction; eauto. *)
-      admit.
-
-    - 
-
-
-
-      
-      (* rewrite Forall_natmap_forall in H0; specialize (H0 _ _ USRS); simpl in H0. *)
-      (* eapply predicates_imply_next_cmd_safe; eauto. *)
-      admit.
-    - admit.
-
-
-    (* pose proof safety_inv. *)
-    (* unfold invariantFor, SYS in H0; simpl in H0. *)
-    (* assert ( (ru0,iu0) = (ru0,iu0) \/ False ) as ARG by eauto. *)
-    (* specialize (H0 _ ARG _ H3). *)
-    (* unfold safety in *; eauto with safe. *)
-
-  Admitted.
+        dt x5; eapply step_na_recur in H12; eauto; split_ex; eauto.
+  Qed.
 
   Hint Resolve simsilent simlabeled simsafe : safe.
 
